code/ecdsap256/Hacl.P256.fst
@@ -28,7 +28,7 @@ open Spec.Hash.Definitions
 open Hacl.Impl.ECDSA.P256.Signature.Agile
 open Hacl.Impl.ECDSA.P256.Verification.Agile
 
-(*
+
 let ecdsa_sign_p256_sha2 result mLen m privKey k = 
   ecdsa_signature P256 (Hash SHA2_256) result mLen m privKey k
 
@@ -73,14 +73,13 @@ let compression_not_compressed_form b result =
 let compression_compressed_form b result = 
   Hacl.Impl.P256.Compression.compressionCompressedForm #P256 b result
 
- 
-
-let reduction_8_32 x result = Hacl.Impl.ECDSA.Reduction.reduction_8_32 #P256 x result 
 
 
-*)
 let ecp256dh_i result scalar = Hacl.Impl.P256.DH.ecp256dh_i P256 result scalar
 
-(*
+let ecp384dh_i result scalar = Hacl.Impl.P256.DH.ecp256dh_i P384 result scalar
+
+
+
 let ecp256dh_r result pubKey scalar = Hacl.Impl.P256.DH.ecp256dh_r P256 result pubKey scalar
-*)
+
